Add proofs about boundedness to GF25519Reflective/Common.v

src/Specific/GF25519Reflective/Common.v
@@ -6,6 +6,7 @@ Require Import Crypto.Reflection.Reify.
 Require Import Crypto.Reflection.Syntax.
 Require Import Crypto.Reflection.Z.Interpretations.
 Require Crypto.Reflection.Z.Interpretations.Relations.
+Require Import Crypto.Reflection.Z.Interpretations.RelationsCombinations.
 Require Import Crypto.Reflection.Z.Reify.
 Require Export Crypto.Reflection.Z.Syntax.
 Require Import Crypto.Reflection.InterpWfRel.
@@ -14,6 +15,7 @@ Require Import Crypto.Reflection.MapInterp.
 Require Import Crypto.Reflection.MapInterpWf.
 Require Import Crypto.Reflection.WfReflective.
 Require Import Crypto.Util.LetIn.
+Require Import Crypto.Util.ZUtil.
 Require Import Crypto.Util.Tactics.
 Require Import Crypto.Util.Notations.
 
@@ -123,6 +125,360 @@ Notation correct_and_bounded_genT ropW'v ropZ_sigv
       /\ interp_type_rel_pointwise2 Relations.related_bounds (Interp (@BoundedWord64.interp_op) ropBoundedWord64) (Interp (@ZBounds.interp_op) ropBounds)
       /\ interp_type_rel_pointwise2 Relations.related_word64 (Interp (@BoundedWord64.interp_op) ropBoundedWord64) (Interp (@Word64.interp_op) ropW))
        (only parsing).
+
+Local Ltac args_to_bounded_helper v :=
+  lazymatch v with
+  | (?x, ?xs)
+    => args_to_bounded_helper x; [ .. | args_to_bounded_helper xs ]
+  | ?w
+    => try refine (_, _); [ refine {| BoundedWord64.value := w |} | .. ]
+  end.
+
+Local Ltac make_args x :=
+  let x' := fresh "x'" in
+  pose (x : id _) as x';
+  cbv [fe25519W wire_digitsW] in x; destruct_head' prod;
+  cbv [fst snd] in *;
+  simpl @fe25519WToZ in *;
+  simpl @wire_digitsWToZ in *;
+  let T := fresh in
+  evar (T : Type);
+  cut T; subst T;
+  [ let H := fresh in
+    intro H;
+    let xv := (eval hnf in x') in
+    args_to_bounded_helper xv;
+    [ destruct_head' and;
+      match goal with
+      | [ H : ?T |- _ ] => is_evar T; refine (proj1 H)
+      end.. ]
+  | repeat match goal with H : is_bounded _ = true |- _ => unfold_is_bounded_in H end;
+    repeat match goal with H : wire_digits_is_bounded _ = true |- _ => unfold_is_bounded_in H end;
+    destruct_head' and;
+    Z.ltb_to_lt;
+    repeat first [ eexact I
+                 | apply conj;
+                   [ repeat apply conj; [ | eassumption | eassumption | ];
+                     vm_compute; [ refine (fun x => match x with eq_refl => I end) | reflexivity ]
+                   | ] ] ].
+
+Local Ltac app_tuples x y :=
+  let tx := type of x in
+  lazymatch (eval hnf in tx) with
+  | prod _ _ => let xs := app_tuples (snd x) y in
+                constr:((fst x, xs))
+  | _ => constr:((x, y))
+  end.
+
+Class is_evar {T} (x : T) := make_is_evar : True.
+Hint Extern 0 (is_evar ?e) => is_evar e; exact I : typeclass_instances.
+
+Definition unop_args_to_bounded (x : fe25519W) (H : is_bounded (fe25519WToZ x) = true)
+  : interp_flat_type (fun _ => BoundedWord64.BoundedWord) (all_binders_for ExprUnOpT).
+Proof. make_args x. Defined.
+Definition unopWireToFE_args_to_bounded (x : wire_digitsW) (H : wire_digits_is_bounded (wire_digitsWToZ x) = true)
+  : interp_flat_type (fun _ => BoundedWord64.BoundedWord) (all_binders_for ExprUnOpWireToFET).
+Proof. make_args x. Defined.
+Definition binop_args_to_bounded (x : fe25519W * fe25519W)
+           (H : is_bounded (fe25519WToZ (fst x)) = true)
+           (H' : is_bounded (fe25519WToZ (snd x)) = true)
+  : interp_flat_type (fun _ => BoundedWord64.BoundedWord) (all_binders_for ExprBinOpT).
+Proof.
+  let v := app_tuples (unop_args_to_bounded (fst x) H) (unop_args_to_bounded (snd x) H') in
+  exact v.
+Defined.
+
+Ltac assoc_right_tuple x so_far :=
+  let t := type of x in
+  lazymatch (eval hnf in t) with
+  | prod _ _ => let so_far := assoc_right_tuple (snd x) so_far in
+                assoc_right_tuple (fst x) so_far
+  | _ => lazymatch so_far with
+         | @None => x
+         | _ => constr:((x, so_far))
+         end
+  end.
+
+Local Ltac make_bounds_prop bounds orig_bounds :=
+  let bounds' := fresh "bounds'" in
+  let bounds_bad := fresh "bounds_bad" in
+  rename bounds into bounds_bad;
+  let boundsv := assoc_right_tuple bounds_bad (@None) in
+  pose boundsv as bounds;
+  pose orig_bounds as bounds';
+  repeat (refine (match fst bounds' with
+                  | Some bounds' => let (l, u) := fst bounds in
+                                    let (l', u') := bounds' in
+                                    ((l' <=? l) && (u <=? u'))%Z%bool
+                  | None => false
+                  end && _)%bool;
+          destruct bounds' as [_ bounds'], bounds as [_ bounds]);
+  try exact (match bounds' with
+             | Some bounds' => let (l, u) := bounds in
+                               let (l', u') := bounds' in
+                               ((l' <=? l) && (u <=? u'))%Z%bool
+             | None => false
+             end).
+
+
+Definition unop_bounds_good (bounds : interp_flat_type (fun _ => ZBounds.bounds) (remove_all_binders ExprUnOpT)) : bool.
+Proof. make_bounds_prop bounds ExprUnOp_bounds. Defined.
+Definition binop_bounds_good (bounds : interp_flat_type (fun _ => ZBounds.bounds) (remove_all_binders ExprBinOpT)) : bool.
+Proof. make_bounds_prop bounds ExprUnOp_bounds. Defined.
+Definition unopFEToWire_bounds_good (bounds : interp_flat_type (fun _ => ZBounds.bounds) (remove_all_binders ExprUnOpFEToWireT)) : bool.
+Proof. make_bounds_prop bounds ExprUnOpWireToFE_bounds. Defined.
+Definition unopWireToFE_bounds_good (bounds : interp_flat_type (fun _ => ZBounds.bounds) (remove_all_binders ExprUnOpWireToFET)) : bool.
+Proof. make_bounds_prop bounds ExprUnOp_bounds. Defined.
+(* TODO FIXME(jgross?, andreser?): Is every function returning a single Z a boolean function? *)
+Definition unopFEToZ_bounds_good (bounds : interp_flat_type (fun _ => ZBounds.bounds) (remove_all_binders ExprUnOpFEToZT)) : bool.
+Proof.
+  refine (let (l, u) := bounds in ((0 <=? l) && (u <=? 1))%Z%bool).
+Defined.
+
+(* FIXME TODO(jgross): This is a horrible tactic.  We should unify the
+    various kinds of correct and boundedness, and abstract in Gallina
+    rather than Ltac *)
+
+Local Ltac t_correct_and_bounded ropZ_sig Hbounds H0 H1 args :=
+  let Heq := fresh "Heq" in
+  let Hbounds0 := fresh "Hbounds0" in
+  let Hbounds1 := fresh "Hbounds1" in
+  let Hbounds2 := fresh "Hbounds2" in
+  pose proof (proj2_sig ropZ_sig) as Heq;
+  cbv [interp_bexpr interp_uexpr interp_uexpr_FEToWire interp_uexpr_FEToZ interp_uexpr_WireToFE
+                    curry_binop_fe25519W curry_unop_fe25519W curry_unop_wire_digitsW
+                    curry_binop_fe25519 curry_unop_fe25519 curry_unop_wire_digits
+                    uncurry_binop_fe25519W uncurry_unop_fe25519W uncurry_unop_wire_digitsW
+                    uncurry_binop_fe25519 uncurry_unop_fe25519 uncurry_unop_wire_digits
+                    ExprBinOpT ExprUnOpFEToWireT ExprUnOpT ExprUnOpFEToZT ExprUnOpWireToFET
+                    interp_type_gen_rel_pointwise interp_type_gen_rel_pointwise] in *;
+  cbv zeta in *;
+  simpl @fe25519WToZ; simpl @wire_digitsWToZ;
+  rewrite <- Heq; clear Heq;
+  destruct Hbounds as [Heq Hbounds];
+  change interp_op with (@Z.interp_op) in *;
+  change interp_base_type with (@Z.interp_base_type) in *;
+  rewrite <- Heq; clear Heq;
+  destruct Hbounds as [ Hbounds0 [Hbounds1 Hbounds2] ];
+  pose proof (fun pf => Relations.uncurry_interp_type_rel_pointwise2_proj_from_option2 Word64.to_Z pf Hbounds2 Hbounds0) as Hbounds_left;
+  pose proof (fun pf => Relations.uncurry_interp_type_rel_pointwise2_proj1_from_option2 Relations.related_word64_boundsi' pf Hbounds1 Hbounds2) as Hbounds_right;
+  specialize_by repeat first [ progress intros
+                             | reflexivity
+                             | assumption
+                             | progress destruct_head' base_type
+                             | progress destruct_head' BoundedWord64.BoundedWord
+                             | progress destruct_head' and
+                             | progress repeat apply conj ];
+  specialize (Hbounds_left args H0);
+  specialize (Hbounds_right args H0);
+  cbv beta in *;
+  lazymatch type of Hbounds_right with
+  | match ?e with _ => _ end
+    => lazymatch type of H1 with
+       | match ?e' with _ => _ end
+         => change e' with e in H1; destruct e eqn:?; [ | exfalso; assumption ]
+       end
+  end;
+  repeat match goal with x := _ |- _ => subst x end;
+  cbv [id
+         binop_args_to_bounded unop_args_to_bounded unopWireToFE_args_to_bounded
+         Relations.proj_eq_rel interp_flat_type_rel_pointwise2 SmartVarfMap interp_flat_type smart_interp_flat_map Application.all_binders_for fst snd BoundedWord64.to_word64' BoundedWord64.boundedWordToWord64 BoundedWord64.value Application.ApplyInterpedAll Application.fst_binder Application.snd_binder interp_flat_type_rel_pointwise2_gen_Prop Relations.related_word64_boundsi' Relations.related'_word64_bounds ZBounds.upper ZBounds.lower Application.remove_all_binders Word64.to_Z] in Hbounds_left, Hbounds_right;
+  match goal with
+  | [ |- fe25519WToZ ?x = _ /\ _ ]
+    => destruct x; destruct_head_hnf' prod
+  | [ |- wire_digitsWToZ ?x = _ /\ _ ]
+    => destruct x; destruct_head_hnf' prod
+  | [ |- _ = _ ]
+    => exact Hbounds_left
+  end;
+  change word64ToZ with Word64.word64ToZ in *;
+  (split; [ exact Hbounds_left | ]);
+  cbv [interp_flat_type] in *;
+  cbv [fst snd
+           binop_bounds_good unop_bounds_good unopFEToWire_bounds_good unopWireToFE_bounds_good unopFEToZ_bounds_good
+           ExprUnOp_bounds ExprBinOp_bounds ExprUnOpFEToWire_bounds ExprUnOpFEToZ_bounds ExprUnOpWireToFE_bounds] in H1;
+  destruct_head' ZBounds.bounds;
+  unfold_is_bounded_in H1;
+  simpl @fe25519WToZ; simpl @wire_digitsWToZ;
+  unfold_is_bounded;
+  destruct_head' and;
+  Z.ltb_to_lt;
+  change Word64.word64ToZ with word64ToZ in *;
+  repeat apply conj; Z.ltb_to_lt; try omega; try reflexivity.
+
+Local Opaque Interp.
+Lemma ExprBinOp_correct_and_bounded
+      ropW op (ropZ_sig : rexpr_binop_sig op)
+      (Hbounds : correct_and_bounded_genT ropW ropZ_sig)
+      (H0 : forall x y
+                   (Hx : is_bounded (fe25519WToZ x) = true)
+                   (Hy : is_bounded (fe25519WToZ y) = true),
+          let args := binop_args_to_bounded (x, y) Hx Hy in
+          match LiftOption.of'
+                  (ApplyInterpedAll (Interp (@BoundedWord64.interp_op) (MapInterp BoundedWord64.of_word64 ropW))
+                                    (LiftOption.to' (Some args)))
+          with
+          | Some _ => True
+          | None => False
+          end)
+      (H1 : forall x y
+                   (Hx : is_bounded (fe25519WToZ x) = true)
+                   (Hy : is_bounded (fe25519WToZ y) = true),
+          let args := binop_args_to_bounded (x, y) Hx Hy in
+          let x' := SmartVarfMap (fun _ : base_type => BoundedWord64.to_bounds') args in
+          match LiftOption.of'
+                  (ApplyInterpedAll (Interp (@ZBounds.interp_op) (MapInterp ZBounds.of_word64 ropW)) (LiftOption.to' (Some x')))
+          with
+          | Some bounds => binop_bounds_good bounds = true
+          | None => False
+          end)
+  : binop_correct_and_bounded (MapInterp (fun _ x => x) ropW) op.
+Proof.
+  intros x y Hx Hy.
+  pose x as x'; pose y as y'.
+  specialize (H0 x' y' Hx Hy).
+  specialize (H1 x' y' Hx Hy).
+  hnf in x, y; destruct_head' prod.
+  let args := constr:(binop_args_to_bounded (x', y') Hx Hy) in
+  t_correct_and_bounded ropZ_sig Hbounds H0 H1 args.
+Qed.
+
+
+Lemma ExprUnOp_correct_and_bounded
+      ropW op (ropZ_sig : rexpr_unop_sig op)
+      (Hbounds : correct_and_bounded_genT ropW ropZ_sig)
+      (H0 : forall x
+                   (Hx : is_bounded (fe25519WToZ x) = true),
+          let args := unop_args_to_bounded x Hx in
+          match LiftOption.of'
+                  (ApplyInterpedAll (Interp (@BoundedWord64.interp_op) (MapInterp BoundedWord64.of_word64 ropW))
+                                    (LiftOption.to' (Some args)))
+          with
+          | Some _ => True
+          | None => False
+          end)
+      (H1 : forall x
+                   (Hx : is_bounded (fe25519WToZ x) = true),
+          let args := unop_args_to_bounded x Hx in
+          let x' := SmartVarfMap (fun _ : base_type => BoundedWord64.to_bounds') args in
+          match LiftOption.of'
+                  (ApplyInterpedAll (Interp (@ZBounds.interp_op) (MapInterp ZBounds.of_word64 ropW)) (LiftOption.to' (Some x')))
+          with
+          | Some bounds => unop_bounds_good bounds = true
+          | None => False
+          end)
+  : unop_correct_and_bounded (MapInterp (fun _ x => x) ropW) op.
+Proof.
+  intros x Hx.
+  pose x as x'.
+  specialize (H0 x' Hx).
+  specialize (H1 x' Hx).
+  hnf in x; destruct_head' prod.
+  let args := constr:(unop_args_to_bounded x' Hx) in
+  t_correct_and_bounded ropZ_sig Hbounds H0 H1 args.
+Qed.
+
+Lemma ExprUnOpFEToWire_correct_and_bounded
+      ropW op (ropZ_sig : rexpr_unop_FEToWire_sig op)
+      (Hbounds : correct_and_bounded_genT ropW ropZ_sig)
+      (H0 : forall x
+                   (Hx : is_bounded (fe25519WToZ x) = true),
+          let args := unop_args_to_bounded x Hx in
+          match LiftOption.of'
+                  (ApplyInterpedAll (Interp (@BoundedWord64.interp_op) (MapInterp BoundedWord64.of_word64 ropW))
+                                    (LiftOption.to' (Some args)))
+          with
+          | Some _ => True
+          | None => False
+          end)
+      (H1 : forall x
+                   (Hx : is_bounded (fe25519WToZ x) = true),
+          let args := unop_args_to_bounded x Hx in
+          let x' := SmartVarfMap (fun _ : base_type => BoundedWord64.to_bounds') args in
+          match LiftOption.of'
+                  (ApplyInterpedAll (Interp (@ZBounds.interp_op) (MapInterp ZBounds.of_word64 ropW)) (LiftOption.to' (Some x')))
+          with
+          | Some bounds => unopFEToWire_bounds_good bounds = true
+          | None => False
+          end)
+  : unop_FEToWire_correct_and_bounded (MapInterp (fun _ x => x) ropW) op.
+Proof.
+  intros x Hx.
+  pose x as x'.
+  specialize (H0 x' Hx).
+  specialize (H1 x' Hx).
+  hnf in x; destruct_head' prod.
+  let args := constr:(unop_args_to_bounded x' Hx) in
+  t_correct_and_bounded ropZ_sig Hbounds H0 H1 args.
+Qed.
+
+Lemma ExprUnOpWireToFE_correct_and_bounded
+      ropW op (ropZ_sig : rexpr_unop_WireToFE_sig op)
+      (Hbounds : correct_and_bounded_genT ropW ropZ_sig)
+      (H0 : forall x
+                   (Hx : wire_digits_is_bounded (wire_digitsWToZ x) = true),
+          let args := unopWireToFE_args_to_bounded x Hx in
+          match LiftOption.of'
+                  (ApplyInterpedAll (Interp (@BoundedWord64.interp_op) (MapInterp BoundedWord64.of_word64 ropW))
+                                    (LiftOption.to' (Some args)))
+          with
+          | Some _ => True
+          | None => False
+          end)
+      (H1 : forall x
+                   (Hx : wire_digits_is_bounded (wire_digitsWToZ x) = true),
+          let args := unopWireToFE_args_to_bounded x Hx in
+          let x' := SmartVarfMap (fun _ : base_type => BoundedWord64.to_bounds') args in
+          match LiftOption.of'
+                  (ApplyInterpedAll (Interp (@ZBounds.interp_op) (MapInterp ZBounds.of_word64 ropW)) (LiftOption.to' (Some x')))
+          with
+          | Some bounds => unopWireToFE_bounds_good bounds = true
+          | None => False
+          end)
+  : unop_WireToFE_correct_and_bounded (MapInterp (fun _ x => x) ropW) op.
+Proof.
+  intros x Hx.
+  pose x as x'.
+  specialize (H0 x' Hx).
+  specialize (H1 x' Hx).
+  hnf in x; destruct_head' prod.
+  let args := constr:(unopWireToFE_args_to_bounded x' Hx) in
+  t_correct_and_bounded ropZ_sig Hbounds H0 H1 args.
+Qed.
+
+Lemma ExprUnOpFEToZ_correct_and_bounded
+      ropW op (ropZ_sig : rexpr_unop_FEToZ_sig op)
+      (Hbounds : correct_and_bounded_genT ropW ropZ_sig)
+      (H0 : forall x
+                   (Hx : is_bounded (fe25519WToZ x) = true),
+          let args := unop_args_to_bounded x Hx in
+          match LiftOption.of'
+                  (ApplyInterpedAll (Interp (@BoundedWord64.interp_op) (MapInterp BoundedWord64.of_word64 ropW))
+                                    (LiftOption.to' (Some args)))
+          with
+          | Some _ => True
+          | None => False
+          end)
+      (H1 : forall x
+                   (Hx : is_bounded (fe25519WToZ x) = true),
+          let args := unop_args_to_bounded x Hx in
+          let x' := SmartVarfMap (fun _ : base_type => BoundedWord64.to_bounds') args in
+          match LiftOption.of'
+                  (ApplyInterpedAll (Interp (@ZBounds.interp_op) (MapInterp ZBounds.of_word64 ropW)) (LiftOption.to' (Some x')))
+          with
+          | Some bounds => unopFEToZ_bounds_good bounds = true
+          | None => False
+          end)
+  : unop_FEToZ_correct (MapInterp (fun _ x => x) ropW) op.
+Proof.
+  intros x Hx.
+  pose x as x'.
+  specialize (H0 x' Hx).
+  specialize (H1 x' Hx).
+  hnf in x; destruct_head' prod.
+  let args := constr:(unop_args_to_bounded x' Hx) in
+  t_correct_and_bounded ropZ_sig Hbounds H0 H1 args.
+Qed.
 
 Ltac rexpr_correct :=
   let ropW' := fresh in
